
%(BEGIN_QUESTION)
% Copyright 2006, Tony R. Kuphaldt, released under the Creative Commons Attribution License (v 1.0)
% This means you may do almost anything with this work of mine, so long as you give me proper credit

Solve for $x$, $y$, and $z$ in this simultaneous system of equations:

$$x + 3y + 5z = 19$$

$$4x - y + 2z = 3$$

$$4x - y - z = 6$$

\vfil 

\underbar{file i00931}
\eject
%(END_QUESTION)





%(BEGIN_ANSWER)

This is a graded question -- no answers or hints given!

%(END_ANSWER)





%(BEGIN_NOTES)

If we take the third equation's terms and subtract them all from the second equation, we arrive at:

$$4x - y + 2z - (4x - y - z) = 3 - (6)$$

$$4x - y + 2z - 4x + y + z = 3 - 6$$

$$3z = -3$$

$$z = -1$$

Plugging this result into the three original equations removes one unknown and leaves us with:

$$x + 3y - 5 = 19$$

$$4x - y - 2 = 3$$

$$4x - y + 1 = 6$$

\vskip 10pt

$$x + 3y = 24$$

$$4x - y = 5$$

\vskip 10pt

We may now solve for $x$ in terms of $y$ (manipulating the first equation), and then plug this definition for $x$ into the second equation to reduce it down to only one variable ($y$):

$$x + 3y = 24 \hskip 30pt x = 24 - 3y$$

$$4x - y = 5$$

$$4(24 - 3y) - y = 5$$

$$96 - 12y - y = 5$$

$$91 = 13y$$

$$y = 7$$

\filbreak

Now that we have a solution for $y$, we may plug the known value for $y$ into the equation $x = 24 - 3y$ and solve for $x$:

$$x = 24 - 3y$$

$$x = 24 - 3(7)$$

$$x = 24 - 21$$

$$x = 3$$

\vskip 10pt

Therefore, $x$ = 3, $y$ = 7, and $z$ = -1

%INDEX% Mathematics review: simultaneous equations

%(END_NOTES)


