
%(BEGIN_QUESTION)
% Copyright 2012, Tony R. Kuphaldt, released under the Creative Commons Attribution License (v 1.0)
% This means you may do almost anything with this work of mine, so long as you give me proper credit

In this series of algebraic steps there is a {\bf mistake}.  Find the mistake and correct it (as well as all subsequent steps):

$$5a - 6ac = 1 - 3a^2b$$

$${{5a - 6ac} \over a} = {{1 - 3a^2b} \over a}$$

$$5 - 6c = 1 - 3ab$$

$$3ab + 5 - 6c = 1$$

\underbar{file i01326}
%(END_QUESTION)





%(BEGIN_ANSWER)

A mistake was made between the second and third equations.  Here is the correction:

$$5a - 6ac = 1 - 3a^2b$$

$${{5a - 6ac} \over a} = {{1 - 3a^2b} \over a}$$

$$5 - 6c = {1 \over a} - 3ab$$

$$3ab + 5 - 6c = {1 \over a}$$

%(END_ANSWER)





%(BEGIN_NOTES)

Students often make the mistake of incomplete division of terms: when additive or subtractive terms are divided by a single term in the denominator, the division extends to each term in the numerator, not just one!

%INDEX% Mathematics review: basic principles of algebra

%(END_NOTES)


